theories/Factor_Complete_Data_Walks.thy
@@ -1,0 +1,260 @@
+theory Factor_Complete_Data_Walks
+  imports Factor_Finite_Prepared_Data_Readings RRA_Executable_Records Finite_Sorted_Set_Execution
+    "HOL-Library.List_Lexorder" "HOL-Library.Product_Lexorder"
+begin
+
+section \<open>A formed data reading is a walk over unique leaves and records\<close>
+
+definition finite_data_leaf_values :: "finite_exact_artifact \<Rightarrow> local_address \<Rightarrow> octets fset" where
+  "finite_data_leaf_values C r=ffilter (finite_payload_leaf_body C r) (finite_payload_values C r)"
+
+lemma finite_data_leaf_values_unique:
+  assumes "v |\<in>| finite_data_leaf_values C r" "w |\<in>| finite_data_leaf_values C r"
+  shows "v=w"
+proof -
+  have "payload_at (decode_finite_object C) r v" "payload_at (decode_finite_object C) r w"
+    using assms by (simp_all add: finite_data_leaf_values_def finite_payload_leaf_body_def finite_payload_at_correct)
+  then show ?thesis by (rule payload_at_unique)
+qed
+
+lemma finite_data_leaf_values_cases:
+  "finite_data_leaf_values C r={||} \<or> (\<exists>v. finite_data_leaf_values C r={|v|})"
+proof (cases "finite_data_leaf_values C r={||}")
+  case False
+  then obtain v where member: "v |\<in>| finite_data_leaf_values C r" by auto
+  have "finite_data_leaf_values C r={|v|}"
+  proof (rule fset_eqI)
+    fix w
+    show "w |\<in>| finite_data_leaf_values C r \<longleftrightarrow> w |\<in>| {|v|}"
+      using finite_data_leaf_values_unique[OF _ member, of w] member by blast
+  qed
+  then show ?thesis by blast
+qed simp
+
+lemma finite_data_leaf_excludes_record:
+  assumes "v |\<in>| finite_data_leaf_values C r"
+  shows "finite_record_body_candidates C r 2={||}"
+proof -
+  have "finite_headed_incidence (finite_structure C) r={||}"
+    using assms by (simp add: finite_data_leaf_values_def finite_payload_leaf_body_def)
+  then show ?thesis by (simp add: finite_record_body_candidates_def Let_def fcard.rep_eq)
+qed
+
+lemma finite_data_record_cases:
+  assumes object: "finite_object_formed C"
+  shows "finite_record_body_candidates C r 2={||} \<or>
+    (\<exists>ps l q. finite_record_body_candidates C r 2={|(ps,[l,q])|} \<and> distinct ps \<and> r\<notin>set ps)"
+proof (cases "finite_record_body_candidates C r 2={||}")
+  case False
+  then obtain ps xs where member: "(ps,xs) |\<in>| finite_record_body_candidates C r 2" by auto
+  have candidate: "(ps,xs) |\<in>| finite_record_candidates C r 2"
+    using member by (simp add: finite_record_body_candidates_exact[OF object])
+  have read: "record_at (decode_finite_object C) r ps xs" and length: "length xs=2"
+    using candidate by (simp_all add: finite_record_candidates_correct)
+  obtain l q where fields: "xs=[l,q]"
+    using length by (cases xs rule: list.exhaust; cases "tl xs" rule: list.exhaust) auto
+  have sockets: "distinct ps" "r\<notin>set ps"
+    using record_at_preserves_socket_occurrences[OF read] by simp_all
+  have only: "finite_record_body_candidates C r 2={|(ps,xs)|}"
+  proof (rule fset_eqI)
+    fix c
+    show "c |\<in>| finite_record_body_candidates C r 2 \<longleftrightarrow> c |\<in>| {|(ps,xs)|}"
+    proof
+      assume "c |\<in>| finite_record_body_candidates C r 2"
+      then obtain qs ys where c: "c=(qs,ys)" and other: "(qs,ys) |\<in>| finite_record_candidates C r 2"
+        by (cases c) (simp add: finite_record_body_candidates_exact[OF object])
+      show "c |\<in>| {|(ps,xs)|}"
+        using finite_record_candidates_unique[OF candidate other] c by simp
+    qed (use member in simp)
+  qed
+  show ?thesis using only fields sockets by blast
+qed simp
+
+lemma finite_singleton_listing [simp]: "sorted_list_of_fset {|x|}=[x]"
+  by (simp add: sorted_list_of_fset.rep_eq)
+
+lemma finite_empty_listing [simp]: "sorted_list_of_fset {||}=[]"
+  by (simp add: sorted_list_of_fset.rep_eq)
+
+fun finite_data_walk :: "nat \<Rightarrow> finite_exact_artifact \<Rightarrow> local_address \<Rightarrow>
+    (finite_factor_term \<times> local_address list) option" where
+  "finite_data_walk 0 C r=None"
+| "finite_data_walk (Suc n) C r=(case sorted_list_of_fset (finite_data_leaf_values C r) of
+      v#vs \<Rightarrow> Some (Finite_Payload v,[r])
+    | [] \<Rightarrow> (case sorted_list_of_fset (finite_record_body_candidates C r 2) of
+        (ps,xs)#rest \<Rightarrow> (case xs of
+            [l,q] \<Rightarrow> (case finite_data_walk n C l of None \<Rightarrow> None
+              | Some (x,ls) \<Rightarrow> (case finite_data_walk n C q of None \<Rightarrow> None
+                | Some (y,qs) \<Rightarrow> Some (Finite_Pair x y,r#ps@ls@qs)))
+          | _ \<Rightarrow> None)
+      | [] \<Rightarrow> None))"
+
+definition finite_walk_readings ::
+  "(finite_factor_term \<times> local_address list) option \<Rightarrow> finite_factor_term finite_syntax_reading fset" where
+  "finite_walk_readings w=(case w of None \<Rightarrow> {||}
+    | Some (t,zs) \<Rightarrow> if distinct zs then {|(t,fset_of_list zs,{||})|} else {||})"
+
+lemma finite_walk_join:
+  assumes sockets: "distinct ps" "r\<notin>set ps"
+  shows "finite_join_readings Finite_Pair {||} r ps (finite_walk_readings (Some (x,ls)))
+      (finite_walk_readings (Some (y,qs)))=finite_walk_readings (Some (Finite_Pair x y,r#ps@ls@qs))"
+proof (cases "distinct ls \<and> distinct qs")
+  case True
+  have disjoint: "finsert r (fset_of_list ps) |\<inter>| (fset_of_list ls |\<union>| fset_of_list qs)={||} \<and>
+      fset_of_list ls |\<inter>| fset_of_list qs={||} \<longleftrightarrow> distinct (r#ps@ls@qs)"
+    using True sockets by (auto simp: fset_eq_iff fset_of_list_elem)
+  have interior: "finsert r (fset_of_list ps) |\<union>| fset_of_list ls |\<union>| fset_of_list qs=fset_of_list (r#ps@ls@qs)"
+    by (auto simp: fset_eq_iff fset_of_list_elem)
+  have join: "finite_join_readings Finite_Pair {||} r ps (finite_walk_readings (Some (x,ls)))
+      (finite_walk_readings (Some (y,qs)))=
+    (if finsert r (fset_of_list ps) |\<inter>| (fset_of_list ls |\<union>| fset_of_list qs)={||} \<and>
+        fset_of_list ls |\<inter>| fset_of_list qs={||}
+      then {|(Finite_Pair x y,finsert r (fset_of_list ps) |\<union>| fset_of_list ls |\<union>| fset_of_list qs,{||})|}
+      else {||})"
+    using True by (simp add: finite_walk_readings_def finite_join_readings_def Let_def)
+  show ?thesis
+    unfolding join disjoint interior by (simp add: finite_walk_readings_def)
+next
+  case False
+  then show ?thesis by (auto simp: finite_walk_readings_def finite_join_readings_def)
+qed
+
+theorem finite_data_walk_readings:
+  assumes formed: "finite_exact_formed C"
+  shows "finite_data_body_readings n C r=finite_walk_readings (finite_data_walk n C r)"
+proof (induction n arbitrary: r)
+  case 0
+  then show ?case by (simp add: finite_walk_readings_def)
+next
+  case (Suc n)
+  have object: "finite_object_formed C" using formed by (simp add: finite_exact_formed_def)
+  have readings: "finite_data_body_readings (Suc n) C r=
+      fimage (\<lambda>v. (Finite_Payload v,{|r|},{||})) (finite_data_leaf_values C r) |\<union>|
+      ffUnion (fimage (\<lambda>(ps,xs). case xs of [l,q] \<Rightarrow>
+        finite_join_readings Finite_Pair {||} r ps (finite_walk_readings (finite_data_walk n C l))
+          (finite_walk_readings (finite_data_walk n C q)) | _ \<Rightarrow> {||})
+        (finite_record_body_candidates C r 2))"
+  proof -
+    have previous: "finite_data_body_readings n C=(\<lambda>q. finite_walk_readings (finite_data_walk n C q))"
+      by (rule ext) (rule Suc.IH)
+    show ?thesis
+      by (simp only: finite_data_body_readings.simps finite_payload_body_readings_def
+        finite_record_body_readings_def finite_data_leaf_values_def previous)
+  qed
+  have claim: "fimage (\<lambda>v. (Finite_Payload v,{|r|},{||})) (finite_data_leaf_values C r) |\<union>|
+      ffUnion (fimage (\<lambda>(ps,xs). case xs of [l,q] \<Rightarrow>
+        finite_join_readings Finite_Pair {||} r ps (finite_walk_readings (finite_data_walk n C l))
+          (finite_walk_readings (finite_data_walk n C q)) | _ \<Rightarrow> {||})
+        (finite_record_body_candidates C r 2))=finite_walk_readings (finite_data_walk (Suc n) C r)"
+  proof (cases "finite_data_leaf_values C r={||}")
+    case False
+    then obtain v where leaf: "finite_data_leaf_values C r={|v|}"
+      using finite_data_leaf_values_cases by blast
+    have none: "finite_record_body_candidates C r 2={||}"
+      by (rule finite_data_leaf_excludes_record[of v]) (simp add: leaf)
+    show ?thesis by (simp add: leaf none finite_walk_readings_def)
+  next
+    case True
+    note empty_leaf=True
+    show ?thesis
+    proof (cases "finite_record_body_candidates C r 2={||}")
+      case True
+      then show ?thesis using empty_leaf by (simp add: finite_walk_readings_def)
+    next
+      case False
+      then obtain ps l q where candidate: "finite_record_body_candidates C r 2={|(ps,[l,q])|}"
+        and sockets: "distinct ps" "r\<notin>set ps"
+        using finite_data_record_cases[OF object] by blast
+      show ?thesis
+      proof (cases "finite_data_walk n C l")
+        case None
+        then show ?thesis
+          using empty_leaf by (simp add: candidate finite_walk_readings_def finite_join_readings_def)
+      next
+        case (Some left)
+        obtain x ls where left: "finite_data_walk n C l=Some (x,ls)" using Some by (cases left) auto
+        show ?thesis
+        proof (cases "finite_data_walk n C q")
+          case None
+          then show ?thesis
+            using empty_leaf left by (simp add: candidate finite_walk_readings_def finite_join_readings_def)
+        next
+          case (Some right)
+          obtain y qs where right: "finite_data_walk n C q=Some (y,qs)" using Some by (cases right) auto
+          show ?thesis
+            using empty_leaf left right finite_walk_join[OF sockets, of x ls y qs]
+            by (simp add: candidate)
+        qed
+      qed
+    qed
+  qed
+  show ?case by (simp only: readings claim)
+qed
+
+section \<open>A complete data reading checks its walk once\<close>
+
+lemma finite_listing_distinct_carrier:
+  "distinct zs \<and> fset_of_list zs=A \<longleftrightarrow> (let s=sort zs in ascending_listing s \<and> s=sorted_list_of_fset A)"
+proof
+  assume walk: "distinct zs \<and> fset_of_list zs=A"
+  have ascending: "ascending_listing (sort zs)"
+    using walk by (simp add: ascending_listing_exact)
+  have carrier: "A=fset_of_list zs" using walk by simp
+  have listing: "sort zs=sorted_list_of_fset A"
+  proof (rule sorted_distinct_set_unique)
+    show "sorted (sort zs)" by simp
+    show "distinct (sort zs)" using walk by simp
+    show "sorted (sorted_list_of_fset A)" by (simp add: sorted_list_of_fset.rep_eq)
+    show "distinct (sorted_list_of_fset A)" by (simp add: sorted_list_of_fset.rep_eq)
+    show "set (sort zs)=set (sorted_list_of_fset A)"
+      by (simp add: carrier sorted_list_of_fset.rep_eq fset_of_list.rep_eq)
+  qed
+  show "let s=sort zs in ascending_listing s \<and> s=sorted_list_of_fset A"
+    using ascending listing by (simp add: Let_def)
+next
+  assume listed: "let s=sort zs in ascending_listing s \<and> s=sorted_list_of_fset A"
+  have ascending: "ascending_listing (sort zs)" using listed unfolding Let_def by blast
+  have listing: "sort zs=sorted_list_of_fset A" using listed unfolding Let_def by blast
+  have "distinct zs" using ascending by (simp add: ascending_listing_exact)
+  moreover have "fset_of_list zs=A"
+    using arg_cong[OF listing, of set] by (simp add: fset_eq_iff fset_of_list.rep_eq sorted_list_of_fset.rep_eq)
+  ultimately show "distinct zs \<and> fset_of_list zs=A" by simp
+qed
+
+lemma finite_card_listing: "fcard A=length (sorted_list_of_fset A)"
+  by (simp add: fcard.rep_eq sorted_list_of_fset.rep_eq)
+
+declare finite_complete_data_readings_prepared_def[code del]
+
+theorem finite_complete_data_readings_walk_code [code]:
+  "finite_complete_data_readings_prepared C r=(if finite_exact_formed C \<and> r |\<in>| finite_carrier (finite_structure C) then
+    (let carrier=sorted_list_of_fset (finite_carrier (finite_structure C)) in
+      case finite_data_walk (length carrier) C r of None \<Rightarrow> {||}
+      | Some (t,zs) \<Rightarrow> (let s=sort zs in if ascending_listing s \<and> s=carrier then {|t|} else {||}))
+    else {||})"
+proof (cases "finite_exact_formed C \<and> r |\<in>| finite_carrier (finite_structure C)")
+  case True
+  then have formed: "finite_exact_formed C" by simp
+  have body_values: "finite_complete_data_body_values C r=(case finite_data_walk (fcard (finite_carrier (finite_structure C))) C r of
+      None \<Rightarrow> {||} | Some (t,zs) \<Rightarrow> if distinct zs \<and> fset_of_list zs=finite_carrier (finite_structure C) then {|t|} else {||})"
+    by (auto simp: finite_complete_data_body_values_def finite_data_walk_readings[OF formed]
+      finite_walk_readings_def fset_eq_iff split: option.splits)
+  show ?thesis
+    using True by (simp add: finite_complete_data_readings_prepared_def body_values finite_card_listing
+      finite_listing_distinct_carrier Let_def split: option.splits)
+next
+  case False
+  then show ?thesis by (simp only: finite_complete_data_readings_prepared_def if_False)
+qed
+
+text \<open>
+  In a formed artifact a node has at most one payload leaf value and at most one
+  two-field record, and never both. Reading its data therefore follows one walk
+  that lists the root, record ports and child walks, and the original pairwise
+  interior conditions hold exactly when that listing has no repetition. A
+  complete reading sorts the listing once and compares it with the canonical
+  carrier, so node interiors are no longer joined at every record. Every
+  original leaf, record, refusal and complete term is unchanged.
+\<close>
+
+end
